Gnosis/Contrarian/ContrarianMissingInterpretationOptimal.lean
@@ -1,6 +1,6 @@
 
-def MissingInterpretation (_α : Type) : Prop := True
-def OptimalConsensus (_α : Type) : Prop := True
+def MissingInterpretation (_α : Type) : Prop := Nonempty _α
+def OptimalConsensus (_α : Type) : Prop := Nonempty _α
 
 theorem missing_interpretation_optimal_consensus {α : Type}
   (_H1 : MissingInterpretation α) (H2 : OptimalConsensus α) :
