Gnosis/Contrarian/ContrarianStallInducesGenerality.lean
@@ -1,6 +1,6 @@
 
-def ExecutionStall (_α : Type) : Prop := True
-def SystemGenerality (_α : Type) : Prop := True
+def ExecutionStall (_α : Type) : Prop := Nonempty _α
+def SystemGenerality (_α : Type) : Prop := Nonempty _α
 
 theorem stall_induces_generality {α : Type}
   (H1 : ExecutionStall α) (H2 : SystemGenerality α) :
