Gnosis/CrossDomain/CrossDomainExecutionStallMycology.lean
@@ -1,8 +1,8 @@
 
 namespace Gnosis.CrossDomainExecutionStallMycology
 
-def MycelialNetwork (_α : Type) : Prop := True
-def ExecutionStall (_α : Type) : Prop := True
+def MycelialNetwork (_α : Type) : Prop := Nonempty _α
+def ExecutionStall (_α : Type) : Prop := Nonempty _α
 
 theorem mycology_execution_stall_bridge {α : Type}
   (H1 : MycelialNetwork α) (H2 : ExecutionStall α) :
